Diff/NonRobustHyperCriterion.v
@@ -1,0 +1,103 @@
+From mathcomp Require Import all_ssreflect. 
+
+Set Implicit Arguments.
+Unset Printing Implicit Defensive.
+
+Require Import ClassicalExtras.
+Require Import MyNotation.
+Require Import Setoid.
+Require Import FunctionalExtensionality.
+Require Import Setoid. 
+
+Require Import Galois.
+Require Import LanguageModel.
+Require Import TraceModel.
+Require Import Properties.
+Require Import ChainModel.
+Require Import NonRobustDef.
+Require Import NonRobustHyperDef.
+
+Hypothesis prop_extensionality : forall A B : Prop, (A <-> B) -> A = B.
+
+Section SafetyCriterion.
+
+  Variable Source Target: Language.
+  Variable compilation_chain : CompilationChain Source Target.
+
+  (*CA: we don't need a particular structure of traces to define preservation 
+        e.g. traces = values or our defn of traces both make sense
+   *)
+  Variable trace__S trace__T : Set.
+  
+  Local Definition prop__S := prop trace__S.
+  Local Definition prop__T := prop trace__T.
+  Local Definition hprop__S := hprop trace__S.
+  Local Definition hprop__T := hprop trace__T.
+  
+  Variable Source_Semantics : Semantics Source trace__S.
+  Variable Target_Semantics : Semantics Target trace__T. 
+
+  Local Definition sem__S := sem Source_Semantics.
+  Local Definition sem__T := sem Target_Semantics.
+  Local Definition beh__S := beh Source_Semantics.
+  Local Definition beh__T := beh Target_Semantics.  
+  Local Definition prg__S := prg Source.
+  Local Definition prg__T := prg Target.
+  Local Definition sat__S := sat Source_Semantics. 
+  Local Definition sat__T := sat Target_Semantics.
+  Local Definition hsat__S := hsat Source_Semantics. 
+  Local Definition hsat__T := hsat Target_Semantics. 
+  
+  Local Definition cmp := compile_whole Source Target compilation_chain.
+
+  Local Notation "W ↓" := (cmp W) (at level 50).
+
+  Variable rel : trace__S -> trace__T -> Prop.  
+ 
+  Local Definition adjunction :=  induced_connection rel. 
+  
+  Local Definition τ' : prop__S -> prop__T := α adjunction.
+  Local Definition σ' : prop__T -> prop__S := γ adjunction.
+
+  Local Definition rel_adjunction_law : Adjunction_law τ' σ' := adjunction_law adjunction. 
+  
+
+  Local Definition τHP := τHP compilation_chain
+                              Source_Semantics Target_Semantics
+                              τ'.
+  
+  
+  Local Definition σHP := σHP compilation_chain
+                              Source_Semantics Target_Semantics
+                              σ'.
+
+  Definition tilde_HC :=  forall W, beh__T (W ↓) = τ' (beh__S W). 
+                                 
+    
+  Theorem tilde_HC_τHP : tilde_HC <-> τHP.
+  Proof.
+    split.
+    - move => H_tilde W h__S. now exists (beh__S W). 
+    - move => H_τHP W. specialize (H_τHP W (fun π__S => π__S = beh__S W)).
+      have Hfoo : hsat__S W (fun π__S => π__S = beh__S W) by auto.                           
+      destruct (H_τHP Hfoo) as [bs [Heq H]]. subst. exact H.  
+  Qed.
+
+  Theorem tilde_HC_σHP : Insertion_snd τ' σ' ->  tilde_HC <-> σHP.
+  Proof.
+    move => H_ins. split.
+    - rewrite tilde_HC_τHP. by apply: Insetion_τHP_σHP. 
+    - setoid_rewrite contra_σHP => H_σHP W.
+      have Hfoo: ~ hsat__T (W ↓) (fun π__T =>  π__T <> (beh__T (W ↓))) by auto.  
+      specialize (H_σHP W (fun π__T =>  π__T <> (beh__T (W ↓))) Hfoo); clear Hfoo.
+      have Hfoo: ~ (lift τ') ((lift σ')  (fun π__T =>  π__T <> (beh__T (W ↓)))) (τ' (beh__S W)). 
+      { admit. }
+      have Hfoofoo: (lift τ') ((lift σ')  (fun π__T =>  π__T <> (beh__T (W ↓)))) = (fun π__T =>  π__T <> (beh__T (W ↓))).
+      { admit. }
+      move: Hfoo. rewrite Hfoofoo -dne. congruence.   
+  Admitted.     
+    
+         
+      
+      
+End SafetyCriterion. 
