Diff/NonRobustHyperDef.v
@@ -1,0 +1,113 @@
+From mathcomp Require Import all_ssreflect. 
+
+Set Implicit Arguments.
+Unset Printing Implicit Defensive.
+
+Require Import ClassicalExtras.
+Require Import MyNotation.
+Require Import Setoid.
+Require Import FunctionalExtensionality.
+
+Require Import Galois.
+Require Import LanguageModel.
+Require Import TraceModel.
+Require Import Properties.
+Require Import ChainModel.
+
+Hypothesis prop_extensionality : forall A B : Prop, (A <-> B) -> A = B.
+
+Notation "W ↓" := (compile_whole _ _ _ W) (at level 50). 
+
+
+Section Preservation. 
+
+
+  Variable Source Target: Language.
+  Variable compilation_chain : CompilationChain Source Target.
+
+  (*CA: we don't need a particular structure of traces to define preservation 
+        e.g. traces = values or our defn of traces both make sense
+   *)
+  Variable trace__S trace__T : Set.
+  
+  Local Definition prop__S := prop trace__S.
+  Local Definition prop__T := prop trace__T.
+  Local Definition hprop__S := hprop trace__S.
+  Local Definition hprop__T := hprop trace__T.
+  
+  Variable Source_Semantics : Semantics Source trace__S.
+  Variable Target_Semantics : Semantics Target trace__T. 
+
+  Local Definition sem__S := sem Source_Semantics.
+  Local Definition sem__T := sem Target_Semantics.
+  Local Definition beh__S := beh Source_Semantics.
+  Local Definition beh__T := beh Target_Semantics.  
+  Local Definition prg__S := prg Source.
+  Local Definition prg__T := prg Target.
+  Local Definition sat__S := sat Source_Semantics. 
+  Local Definition sat__T := sat Target_Semantics.
+  Local Definition hsat__S := hsat Source_Semantics. 
+  Local Definition hsat__T := hsat Target_Semantics. 
+  
+  Local Definition cmp := compile_whole Source Target compilation_chain.
+
+  Local Notation "W ↓" := (cmp W) (at level 50).
+  
+  Variable σ : prop__T -> prop__S. 
+  Variable τ : prop__S -> prop__T. 
+
+  Local Definition σ__h : hprop__T -> hprop__S := lift σ. 
+  Local Definition τ__h : hprop__S -> hprop__T := lift τ. 
+  
+  Definition σhP (W : prg__S) (h__T : hprop__T) :=
+    hsat__S W (σ__h h__T) -> hsat__T (W ↓) h__T.
+
+  Definition σHP := forall W h__T, σhP W h__T.
+
+  Lemma contra_σhP (W : prg__S) (h__T : hprop__T) :
+    (σhP W h__T) <->  (~  h__T (beh__T (W ↓))  ->
+                  (~  (σ__h h__T) (beh__S W))). 
+  Proof.
+    rewrite /σhP. by rewrite contra.
+  Qed. 
+  
+  Lemma contra_σHP :
+    σHP <-> (forall W h__T,  (~  h__T (beh__T (W ↓))  ->
+                  (~  (σ__h h__T) (beh__S W)))) .
+  Proof.
+    rewrite /σHP. 
+    split => H W h__T; by move/contra_σhP: (H W h__T).
+  Qed.
+
+  Definition τhP (W : prg__S) (h__S : hprop__S) :=
+    hsat__S W h__S -> hsat__T (W ↓) (τ__h h__S).
+
+  Definition τHP := forall W h__S, τhP W h__S.
+
+
+  Lemma contra_τhP (W : prg__S) (h__S : hprop__S) :
+    (τhP W h__S) <->  ((~  (τ__h h__S) (beh__T (W ↓)))  ->
+                  (~   h__S (beh__S W))).
+  Proof.
+    rewrite /τhP. by rewrite contra.  
+  Qed.      
+  
+  Lemma contra_τHP :
+    τHP <-> (forall W h__S,  ((~  (τ__h h__S) (beh__T (W ↓)))  ->
+                     (~   h__S (beh__S W)))).
+  Proof.
+    rewrite /τHP.
+    split => H W h__S; by move/contra_τhP: (H W h__S).
+  Qed.
+  
+  Theorem Insetion_τHP_σHP :
+    (Insertion_snd τ σ) -> (τHP -> σHP).
+  Proof.
+    move => H_in Hτ W h__t H_src.
+    move: (Hτ W (σ__h h__t) H_src) => [b__s [[bt [H_bt Heq]] H_trg]].  
+    subst.
+    have Hfoo : τ (σ bt) = bt by apply: H_in. 
+    by rewrite /hsat__T /hsat H_trg Hfoo.   
+  Qed.     
+
+End Preservation.                                      
